src/Bitstream.v
@@ -2,6 +2,7 @@ Require Import String.
 Require Import AST.
 Require Import List.
 Require Import Values.
+Require Import Semantics.
 
 (* We need easy ways of writing down inputs to cryptol functions *)
 (* They only need base type bit, and structures *)
@@ -139,6 +140,82 @@ Lemma to_val_lp_fst :
 Proof.
   induction f; simpl; intros; auto; destruct a; simpl; f_equal; auto.
 Qed.
+
+Lemma strict_eval_list :
+  forall l ge,
+    Forall (fun v => strict_eval_val ge (to_val v) (to_sval v)) l ->
+    strict_eval_val ge (thunk_list (map to_val l)) (strict_list (map to_sval l)).
+Proof.
+  induction l; intros.
+  simpl. econstructor; eauto.
+  simpl.
+  inversion H. subst. eapply IHl in H3.
+  econstructor; eauto.
+  econstructor; eauto.
+Qed.
+
+Lemma Forall2_map_Forall :
+  forall {A B C : Type} P (f1 : A -> B) (f2 : A -> C) (l : list A),
+    Forall (fun x => P (f1 x) (f2 x)) l ->
+    Forall2 P (map f1 l) (map f2 l).
+Proof.
+  induction 1; intros.
+  simpl. econstructor.
+  simpl. econstructor; eauto.
+Qed.
+
+Lemma separate_combine :
+  forall {A B : Type} (l : list (A * B)),
+    l = combine (map fst l) (map snd l).
+Proof.
+  induction l; intros; simpl; auto.
+  destruct a; simpl; f_equal; eauto.
+Qed.
+
+Lemma strict_eval_rec :
+  forall ge f,
+    Forall (fun ev : ext_val => strict_eval_val ge (to_val ev) (to_sval ev)) (map snd f) ->
+    strict_eval_val ge (to_val (erec f)) (to_sval (erec f)).
+Proof.
+  induction f; intros.
+  simpl.
+  rewrite (@separate_combine string strictval) at 1. econstructor.
+  econstructor. reflexivity.
+
+  simpl in H. inversion H. subst.
+  specialize (IHf H3).
+  destruct a. simpl in H2.
+  simpl. fold to_val_list_pair.
+  fold to_sval_list_pair.
+  econstructor. simpl. econstructor. eassumption.
+  instantiate (1 := (map snd (to_sval_list_pair f))).
+  rewrite map_snd_to_val_lp.
+  rewrite map_snd_to_sval_lp.
+  eapply Forall2_map_Forall.
+  eapply H3.
+  simpl. f_equal.
+  rewrite (separate_combine (to_sval_list_pair f)) at 1.
+  f_equal.
+  rewrite to_val_lp_fst.
+  rewrite to_sval_lp_fst.
+  reflexivity.
+Qed.
+
+Lemma strict_eval_val_to_val :
+  forall ge (ev : ext_val),
+    strict_eval_val ge (to_val ev) (to_sval ev).
+Proof.
+  induction ev using ext_val_ind_mut; intros;
+    try solve [econstructor; eauto].
+  simpl.
+  eapply strict_eval_list; eauto.
+  simpl.
+  econstructor.
+  eapply Forall2_map_Forall; eauto.
+  eapply strict_eval_rec; eauto.
+Qed.
+
+
 
 Inductive ext_type :=
 | tbit
